src/program_proof/twophase/twophase_sub_logical_reln_defs.v
@@ -14,7 +14,10 @@ From Perennial.Helpers Require List.
 
 From Perennial.goose_lang.ffi Require Import jrnl_ffi.
 From Perennial.goose_lang.ffi Require Import disk.
+From Perennial.program_proof Require Import twophase.typed_translate.
 From Perennial.program_proof Require Import twophase.twophase_refinement.
+From Perennial.program_proof Require Import twophase.wrapper_proof.
+From Perennial.program_proof Require buftxn.sep_buftxn_proof.
 
 Set Default Proof Using "Type".
 
@@ -59,20 +62,27 @@ Notation SCtx := (@Ctx (@val_tys _ spec_ty)).
 
 Definition val_semTy `{!heapG Σ} `{refinement_heapG Σ} := sval → ival → iProp Σ.
 
+Import sep_buftxn_invariant.
 Section reln_defs.
 Context `{hG: !heapG Σ}.
+Context `{!buftxnG Σ}.
 Context {hRG: refinement_heapG Σ}.
+Context (N: namespace).
 Context (SIZE: nat).
+Context (dinit : abstraction.disk).
+Context (objs_dom : gset addr_proof.addr).
+Context (γ γ': sep_buftxn_invariant.buftxn_names Σ).
+Context (tph: loc).
 
 
 Existing Instances spec_ffi_model_field (* spec_ext_op_field *) spec_ext_semantics_field (* spec_ffi_interp_field  *) spec_ffi_interp_adequacy_field.
 
-(* XXX: Replace j ↦ K es with an always_steps + the non-persistent resourceses accumulated by
-   twophase ops *)
 Definition atomically_has_semTy (es: sexpr) (e: iexpr) (vty: val_semTy) : iProp Σ :=
-  (∀ (j: nat) (K: sexpr → sexpr) (CTX: LanguageCtx K),
-      j ⤇ K es -∗ WPC e @ (logical_reln_defns.sty_lvl_ops (specTy_model := jrnlTy_model SIZE)); ⊤
-                    {{ v, ∃ vs, j ⤇ K (of_val vs) ∗ vty vs v }} {{ True }})%I.
+  (∀ (j: nat) e0 (K: sexpr → sexpr) (CTX: LanguageCtx' K),
+      is_twophase_started N tph γ γ' dinit objs_dom j e0 (K es) -∗
+      WPC e @ (logical_reln_defns.sty_lvl_ops (specTy_model := jrnlTy_model SIZE)); ⊤
+                    {{ v, ∃ vs, is_twophase_started N tph γ γ' dinit objs_dom j e0 (K (of_val vs)) ∗
+                                vty vs v }} {{ True }})%I.
 
 Definition atomically_base_ty_interp (t: base_ty) :=
   λ (v1: sval) (v2: ival),
@@ -174,7 +184,6 @@ Proof.
   apply big_sepM_persistent => ??. apply atomically_val_interp_pers.
 Qed.
 
-End reln_defs.
 
 (*
 Arguments val_interp {ext ffi ffi_semantics interp spec_ext spec_ffi spec_ffi_semantics spec_interp _ Σ hG hRG
@@ -185,4 +194,772 @@ Arguments ctx_has_semTy {ext ffi ffi_semantics interp spec_ext spec_ffi spec_ffi
 
 Arguments specTy_model {ext ffi interp spec_ext spec_ffi spec_ffi_semantics spec_interp} spec_ty.
 *)
+
+Scheme expr_typing_ind := Induction for atomic_body_expr_transTy Sort Prop with
+    val_typing_ind := Induction for atomic_body_val_transTy Sort Prop.
+
+Lemma disc_crash_true E k :
+  ⊢ <disc> (|C={E}_k=> True).
+Proof. auto. Qed.
+
+Tactic Notation "spec_bind" open_constr(efoc) " as " ident(H) :=
+  iStartProof;
+  lazymatch goal with
+  | |- context[ (is_twophase_started _ _ _ _ _ _ _ _ (?Kinit ?e))%I ] =>
+    let H' := fresh H in
+    refine_reshape_expr e ltac:(fun K' e' => unify e' efoc; destruct (tac_refine_bind' Kinit K' e e') as (->&H'); [split; eauto|])
+    || fail "spec_bind: cannot find" efoc "in" e
+  end.
+
+Lemma ctx_has_semTy_subst
+      e (es: sexpr) (t: sty) x v vs tx Γ:
+      ctx_has_semTy (<[x:=tx]> Γ) es e t -∗
+      atomically_val_interp tx vs v -∗
+      ctx_has_semTy Γ (subst' x vs es) (subst' x v e) t.
+Proof.
+  rewrite /ctx_has_semTy.
+  iIntros "Hhasty Hval".
+  iIntros (Γsubst Hproj) "Hspec Hctx".
+  destruct x as [|x] => //=.
+  { iApply ("Hhasty" with "[] [$] [$]").
+    eauto.
+  }
+  rewrite -?subst_map_insert'.
+  iSpecialize ("Hhasty" $! (<[x := {| subst_ty := tx; subst_sval := vs; subst_ival := v |}]> Γsubst)
+                 with "[] [$] [Hctx Hval]").
+  { iPureIntro. rewrite -Hproj. apply: fmap_insert. }
+  { iPoseProof (big_sepM_insert_2 with "[Hval] [Hctx]") as "$".
+    * iFrame.
+    * eauto.
+  }
+  rewrite ?fmap_insert //=.
+Qed.
+
+Lemma comparableTy_val_eq t vs1 v1 vs2 v2:
+  is_comparableTy t = true →
+  atomically_val_interp t vs1 v1 -∗
+  atomically_val_interp t vs2 v2 -∗
+  ⌜ v1 = v2 ↔ vs1 = vs2 ⌝.
+Proof.
+  revert vs1 v1 vs2 v2.
+  induction t => vs1 v1 vs2 v2; try (inversion 1; fail).
+  - intros. destruct t; iPureIntro; naive_solver.
+  - intros (?&?)%andb_prop.
+    intros.
+    iDestruct 1 as (?? ?? (->&->)) "(H1&H2)".
+    iDestruct 1 as (?? ?? (->&->)) "(H1'&H2')".
+    rewrite -/atomically_val_interp.
+    iPoseProof (IHt1 with "H1 H1'") as "%"; eauto.
+    iPoseProof (IHt2 with "H2 H2'") as "%"; eauto.
+    iPureIntro. naive_solver.
+  - intros (?&?)%andb_prop.
+    intros.
+    iDestruct 1 as "[H|H]";
+    iDestruct 1 as "[H'|H']";
+    iDestruct "H" as (?? (->&->)) "H";
+    iDestruct "H'" as (?? (->&->)) "H'".
+    * iPoseProof (IHt1 with "H H'") as "%"; eauto.
+      iPureIntro. split; inversion 1; subst; f_equal; naive_solver.
+    * iPureIntro; split; inversion 1.
+    * iPureIntro; split; inversion 1.
+    * iPoseProof (IHt2 with "H H'") as "%"; eauto.
+      iPureIntro. split; inversion 1; subst; f_equal; naive_solver.
+  - intros. iIntros "[] H2".
+  - intros. iIntros "[] H2".
+Qed.
+
+Lemma atomically_fundamental_lemma:
+  ∀ Γ (es : sexpr) (e : iexpr) τ, atomic_body_expr_transTy Γ (of_val #tph) es e τ →
+    ⊢ ctx_has_semTy Γ es e τ.
+Proof.
+  iIntros (???? Htyping).
+  remember (of_val #tph) as tph'.
+  revert Heqtph'.
+  induction Htyping using @expr_typing_ind with
+      (P := (λ Γ tph' (es : sexpr) (e : iexpr) τ
+             (HTYPE: atomic_body_expr_transTy Γ tph' es e τ),  tph' = of_val #tph →
+               ⊢ ctx_has_semTy Γ es e τ))
+      (P0 := (λ Γ tph' vs v τ
+             (HTYPE: atomic_body_val_transTy Γ tph' vs v τ), tph' = of_val #tph →
+               ⊢ atomically_val_interp τ vs v)); intros ->;
+      try (iIntros (Γsubst HPROJ) "#Hspec #Hctx";
+           iIntros (j e0 K Hctx) "Hj").
+  - subst.
+    rewrite lookup_fmap in e.
+    apply fmap_Some_1 in e as (t'&?&?). subst.
+    iDestruct (big_sepM_lookup with "Hctx") as "H"; first eauto.
+    rewrite /= ?lookup_fmap H //=.
+    iApply wpc_value; iSplit.
+    * iModIntro. iExists _; iFrame "H"; iFrame.
+    * iApply disc_crash_true.
+  - subst.
+    simpl.
+    iPoseProof (IHHtyping1 with "[//] [$] [$]") as "H"; first done.
+    wpc_bind (subst_map ((subst_ival <$> Γsubst)) x2).
+    spec_bind (subst_map ((subst_sval <$> Γsubst)) x1) as Hctx'.
+    rewrite /atomically_has_semTy.
+    iSpecialize ("H" $! j _ _ Hctx' with "Hj").
+    iApply (wpc_mono' with "[] [] H"); last auto.
+    iIntros (v2) "H". iDestruct "H" as (vs2) "(Hj&Hv2)".
+    wpc_bind (subst_map _ f2).
+    iPoseProof (IHHtyping2 with "[//] [$] [$]") as "H"; first done.
+    iSpecialize ("H" $! j _ (λ x, K (ectx_language.fill [AppLCtx (vs2)] x)) with "[] Hj").
+    { iPureIntro. apply comp_ctx'; last done. apply ectx_lang_ctx'. }
+    iApply (wpc_mono' with "[Hv2] [] H"); last by iModIntro.
+    iIntros (v1) "H". iDestruct "H" as (vs1) "(Hj&Hv1)".
+    simpl. iDestruct "Hv1" as (?????? (Heq1&Heq2)) "#Hinterp".
+    iSpecialize ("Hinterp" $! _ _ with "Hv2").
+    rewrite /atomically_has_semTy.
+    clear Hctx'.
+    iApply ("Hinterp" with "Hj").
+  - subst.
+    iApply wp_wpc. iApply wp_value. iExists _. iFrame.
+    iApply (IHHtyping); auto.
+  - subst. simpl.
+    iApply wp_wpc.
+    iDestruct (twophase_started_step_puredet with "Hj") as "Hj".
+    { intros ?.
+      apply head_prim_step_trans'. econstructor; eauto.
+      { simpl. econstructor; eauto. }
+      { econstructor; eauto. }
+    }
+    wp_pures; eauto.
+    iExists _; iFrame.
+    iExists _, _, _, _, _, _; iSplit; first eauto.
+    iLöb as "IH".
+    iModIntro. iIntros (v vs) "Hval".
+    clear j K Hctx.
+    iIntros (j ? K Hctx) "Hj".
+    wpc_pures.
+    { iClear "∗ #". auto. }
+    iApply wp_wpc.
+    iDestruct (twophase_started_step_puredet with "Hj") as "Hj".
+    { intros ?.
+      apply head_prim_step_trans'. econstructor; eauto.
+    }
+    iPoseProof (ctx_has_semTy_subst with "[] []") as "H1".
+    { iApply IHHtyping. eauto. }
+    { simpl. iExists _, _, _, _, _, _. iFrame "IH"; eauto. }
+    iPoseProof (ctx_has_semTy_subst with "[] Hval") as "H2".
+    { iApply "H1". }
+    iSpecialize ("H2" with "[//] [$] [$] [//] [Hj]").
+    { do 2 (rewrite -subst_map_binder_insert' subst_map_binder_insert).
+      iEval (rewrite (binder_delete_commute f x)). iFrame. }
+    { do 2 (rewrite -subst_map_binder_insert' subst_map_binder_insert).
+      iEval (rewrite {2}binder_delete_commute). iApply wpc_wp. iFrame. }
+  - subst. simpl.
+    iPoseProof (IHHtyping1 with "[//] [$] [$]") as "H"; eauto.
+    wpc_bind (subst_map ((subst_ival <$> Γsubst)) cond').
+    spec_bind (_ _ cond) as Hctx'.
+    iSpecialize ("H" $! j _ _ Hctx' with "Hj").
+    clear Hctx'.
+    iApply (wpc_mono' with "[] [] H"); last auto.
+
+    iIntros (vcond) "H". iDestruct "H" as (vscond) "(Hj&Hvcond)".
+    (* split on the value of the bool *)
+    iDestruct "Hvcond" as %(b&->&->).
+    destruct b.
+    * wpc_pures; first by (iClear "∗ #"; auto). simpl.
+      iApply wp_wpc.
+      iDestruct (twophase_started_step_puredet with "Hj") as "Hj".
+      { intros ?.
+        apply head_prim_step_trans'. econstructor; eauto.
+      }
+      iApply wpc_wp.
+      iApply (IHHtyping2 with "[//] [$] [$]"); eauto.
+    * wpc_pures; first by (iClear "∗ #"; auto). simpl.
+      iApply wp_wpc.
+      iDestruct (twophase_started_step_puredet with "Hj") as "Hj".
+      { intros ?.
+        apply head_prim_step_trans'. econstructor; eauto.
+      }
+      iApply wpc_wp.
+      iApply (IHHtyping3 with "[//] [$] [$]"); eauto.
+  - subst. simpl.
+    iApply wp_wpc.
+    iMod (twophase_started_ub_det with "Hj") as %[]; swap 1 3.
+    { set_solver+. }
+    { intros; eapply stuck_Panic'. }
+  - subst. simpl.
+    iApply wp_wpc.
+    iApply wp_ncfupd.
+    iApply wp_ArbitraryInt; first auto.
+    iNext.
+    iIntros.
+    iDestruct (twophase_started_step_puredet with "Hj") as "Hj".
+    { intros ?.
+      apply head_prim_step_trans'. repeat econstructor; eauto.
+    }
+    iModIntro. iExists _. iFrame. iExists _. iPureIntro; eauto.
+  - subst. simpl.
+    wpc_bind (subst_map _ e2).
+    iPoseProof (IHHtyping with "[//] [$] [$]") as "H"; first auto.
+    iSpecialize ("H" $! j _ (λ x, K (ectx_language.fill [UnOpCtx _] x)) with "[] Hj").
+    { iPureIntro. apply comp_ctx'; last done. apply ectx_lang_ctx'. }
+    iApply (wpc_mono' with "[] [] H"); last by auto.
+    iIntros (v1) "H". iDestruct "H" as (vs1) "(Hj&Hv1)".
+    iAssert (∃ (vres: u64), ⌜ un_op_eval ToUInt64Op v1 = Some #vres ∧
+                            un_op_eval ToUInt64Op vs1 = Some #vres ⌝)%I with "[Hv1]" as %Hres.
+    {
+      destruct t; try inversion e;
+      destruct t; try congruence;
+      rewrite /atomically_val_interp//=;
+      iDestruct "Hv1" as (?) "(%&%)"; subst;
+      iPureIntro; eexists; eauto.
+    }
+    destruct Hres as (x&Heq1&Heq2).
+    iApply wp_wpc.
+    iDestruct (twophase_started_step_puredet with "Hj") as "Hj".
+    { intros ?.
+      apply head_prim_step_trans'. repeat econstructor; eauto.
+        rewrite Heq2; eauto. econstructor; eauto.
+    }
+    wp_pures; eauto.
+  - subst. simpl.
+    wpc_bind (subst_map _ e2).
+    iPoseProof (IHHtyping with "[//] [$] [$]") as "H"; first auto.
+    spec_bind (_ _ e1) as Hctx'.
+    iSpecialize ("H" $! j _ _ Hctx' with "Hj"); clear Hctx'.
+    iApply (wpc_mono' with "[] [] H"); last by auto.
+    iIntros (v1) "H". iDestruct "H" as (vs1) "(Hj&Hv1)".
+    iAssert (∃ (vres: u32), ⌜ un_op_eval ToUInt32Op v1 = Some #vres ∧
+                            un_op_eval ToUInt32Op vs1 = Some #vres ⌝)%I with "[Hv1]" as %Hres.
+    {
+      destruct t; try inversion e;
+      destruct t; try congruence;
+      rewrite /atomically_val_interp//=;
+      iDestruct "Hv1" as (?) "(%&%)"; subst;
+      iPureIntro; eexists; eauto.
+    }
+    destruct Hres as (x&Heq1&Heq2).
+    iApply wp_wpc.
+    iDestruct (twophase_started_step_puredet with "Hj") as "Hj".
+    { intros ?.
+      apply head_prim_step_trans'. repeat econstructor; eauto.
+        rewrite Heq2; eauto. econstructor; eauto.
+    }
+    wp_pures; eauto.
+  - subst. simpl.
+    wpc_bind (subst_map _ e2).
+    iPoseProof (IHHtyping with "[//] [$] [$]") as "H"; first auto.
+    spec_bind (_ _ e1) as Hctx'.
+    iSpecialize ("H" $! j _ _ Hctx' with "Hj"); clear Hctx'.
+    iApply (wpc_mono' with "[] [] H"); last by auto.
+    iIntros (v1) "H". iDestruct "H" as (vs1) "(Hj&Hv1)".
+    iAssert (∃ (vres: u8), ⌜ un_op_eval ToUInt8Op v1 = Some #vres ∧
+                            un_op_eval ToUInt8Op vs1 = Some #vres ⌝)%I with "[Hv1]" as %Hres.
+    {
+      destruct t; try inversion e;
+      destruct t; try congruence;
+      rewrite /atomically_val_interp//=;
+      iDestruct "Hv1" as (?) "(%&%)"; subst;
+      iPureIntro; eexists; eauto.
+    }
+    destruct Hres as (x&Heq1&Heq2).
+    iApply wp_wpc.
+    iDestruct (twophase_started_step_puredet with "Hj") as "Hj".
+    { intros ?.
+      apply head_prim_step_trans'. repeat econstructor; eauto.
+        rewrite Heq2; eauto. econstructor; eauto.
+    }
+    wp_pures; eauto.
+  - subst. simpl.
+    wpc_bind (subst_map _ e2).
+    iPoseProof (IHHtyping with "[//] [$] [$]") as "H"; first auto.
+    spec_bind (_ _ e1) as Hctx'.
+    iSpecialize ("H" $! j _ _ Hctx' with "Hj"); clear Hctx'.
+    iApply (wpc_mono' with "[] [] H"); last by auto.
+    iIntros (v1) "H". iDestruct "H" as (vs1) "(Hj&Hv1)".
+    iAssert (∃ (vres: string), ⌜ un_op_eval ToStringOp v1 = Some #(LitString vres) ∧
+                            un_op_eval ToStringOp vs1 = Some #(LitString vres) ⌝)%I with "[Hv1]" as %Hres.
+    {
+      destruct t; try inversion e;
+      destruct t; try congruence;
+      rewrite /atomically_val_interp//=;
+      iDestruct "Hv1" as (?) "(%&%)"; subst;
+      iPureIntro; eexists; eauto.
+    }
+    destruct Hres as (x&Heq1&Heq2).
+    iApply wp_wpc.
+    iDestruct (twophase_started_step_puredet with "Hj") as "Hj".
+    { intros ?.
+      apply head_prim_step_trans'. repeat econstructor; eauto.
+        rewrite Heq2; eauto. econstructor; eauto.
+    }
+    wp_pures; eauto.
+  - destruct op; try inversion e; subst. simpl.
+    wpc_bind (subst_map _ e2).
+    iPoseProof (IHHtyping with "[//] [$] [$]") as "H"; first auto.
+    spec_bind (_ _ e1) as Hctx'.
+    iSpecialize ("H" $! j _ _ Hctx' with "Hj"); clear Hctx'.
+    iApply (wpc_mono' with "[] [] H"); last by auto.
+    iIntros (v1) "H". iDestruct "H" as (vs1) "(Hj&Hv1)".
+    iDestruct "Hv1" as (?) "(%&%)"; subst.
+    iApply wp_wpc.
+    iDestruct (twophase_started_step_puredet with "Hj") as "Hj".
+    { intros ?.
+      apply head_prim_step_trans'. repeat econstructor; eauto.
+    }
+    wp_pures; eauto.
+  - subst. simpl.
+    iPoseProof (IHHtyping1 with "[//] [$] [$]") as "H"; eauto.
+    wpc_bind (subst_map ((subst_ival <$> Γsubst)) e1').
+    spec_bind (_ _ e1) as Hctx'.
+    iSpecialize ("H" $! j _ _ Hctx' with "Hj"); clear Hctx'.
+    iApply (wpc_mono' with "[] [] H"); last by auto.
+    iIntros (v1) "H". iDestruct "H" as (vs1) "(Hj&Hv1)".
+    wpc_bind (subst_map _ e2').
+    iPoseProof (IHHtyping2 with "[//] [$] [$]") as "H"; eauto.
+    simpl. spec_bind (_ _ e2) as Hctx'.
+    iSpecialize ("H" $! j _ _ Hctx' with "Hj"); clear Hctx'.
+    iApply (wpc_mono' with "[Hv1] [] H"); last by auto.
+    iIntros (v2) "H". iDestruct "H" as (vs2) "(Hj&Hv2)".
+    iApply wp_wpc.
+    iDestruct (twophase_started_step_puredet with "Hj") as "Hj".
+    { intros ?.
+      apply head_prim_step_trans'. repeat econstructor; eauto.
+    }
+    wp_pures; auto.
+    iExists _. iFrame. iExists (bool_decide (vs1 = vs2)); eauto.
+    iDestruct (comparableTy_val_eq with "Hv1 Hv2") as %Heq; auto.
+    iPureIntro. split; first auto. do 2 f_equal.
+    by apply bool_decide_iff.
+  - subst. simpl.
+    wpc_bind (subst_map _ e1').
+    iPoseProof (IHHtyping1 with "[//] [$] [$]") as "H"; eauto.
+    spec_bind (_ _ e1) as Hctx'.
+    iSpecialize ("H" $! j _ _ Hctx' with "Hj"); clear Hctx'.
+    iApply (wpc_mono' with "[] [] H"); last by auto.
+    iIntros (v1) "H". iDestruct "H" as (vs1) "(Hj&Hv1)".
+    simpl.
+
+    wpc_bind (subst_map _ e2').
+    iPoseProof (IHHtyping2 with "[//] [$] [$]") as "H"; eauto.
+    spec_bind (_ _ e2) as Hctx'.
+    iSpecialize ("H" $! j _ _ Hctx' with "Hj"); clear Hctx'.
+    iApply (wpc_mono' with "[Hv1] [] H"); last by auto.
+    iIntros (v2) "H". iDestruct "H" as (vs2) "(Hj&Hv2)".
+    simpl.
+
+    iDestruct "Hspec" as "(#Hsrc&#Hstate)".
+    (* Be patient, this is handling a bunch of cases. *)
+    iApply wp_wpc.
+    destruct op; inversion e; subst;
+      iDestruct "Hv1" as (?) "(%&%)"; subst;
+      iDestruct "Hv2" as (?) "(%&%)"; subst;
+    (iDestruct (twophase_started_step_puredet with "Hj") as "Hj";
+        [ intros ?; apply head_prim_step_trans'; repeat econstructor; eauto
+        | wp_pures; eauto; iExists _; iFrame; eauto]).
+  - subst. simpl.
+    wpc_bind (subst_map _ e1').
+    iPoseProof (IHHtyping1 with "[//] [$] [$]") as "H"; eauto.
+    spec_bind (_ _ e1) as Hctx'.
+    iSpecialize ("H" $! j _ _ Hctx' with "Hj"); clear Hctx'.
+    iApply (wpc_mono' with "[] [] H"); last by auto.
+    iIntros (v1) "H". iDestruct "H" as (vs1) "(Hj&Hv1)".
+    simpl.
+
+    wpc_bind (subst_map _ e2').
+    iPoseProof (IHHtyping2 with "[//] [$] [$]") as "H"; eauto.
+    spec_bind (_ _ e2) as Hctx'.
+    iSpecialize ("H" $! j _ _ Hctx' with "Hj"); clear Hctx'.
+    iApply (wpc_mono' with "[Hv1] [] H"); last by auto.
+    iIntros (v2) "H". iDestruct "H" as (vs2) "(Hj&Hv2)".
+    simpl.
+
+    iDestruct "Hspec" as "(#Hsrc&#Hstate)".
+    (* Be patient, this is handling a bunch of cases. *)
+    iApply wp_wpc.
+    destruct op; inversion e; subst;
+      iDestruct "Hv1" as (?) "(%&%)"; subst;
+      iDestruct "Hv2" as (?) "(%&%)"; subst;
+    (iDestruct (twophase_started_step_puredet with "Hj") as "Hj";
+        [ intros ?; apply head_prim_step_trans'; repeat econstructor; eauto
+        | wp_pures; eauto; iExists _; iFrame; eauto]).
+  - subst. simpl.
+    wpc_bind (subst_map _ e1').
+    iPoseProof (IHHtyping1 with "[//] [$] [$]") as "H"; eauto.
+    spec_bind (_ _ e1) as Hctx'.
+    iSpecialize ("H" $! j _ _ Hctx' with "Hj"); clear Hctx'.
+    iApply (wpc_mono' with "[] [] H"); last by auto.
+    iIntros (v1) "H". iDestruct "H" as (vs1) "(Hj&Hv1)".
+    simpl.
+
+    wpc_bind (subst_map _ e2').
+    iPoseProof (IHHtyping2 with "[//] [$] [$]") as "H"; eauto.
+    spec_bind (_ _ e2) as Hctx'.
+    iSpecialize ("H" $! j _ _ Hctx' with "Hj"); clear Hctx'.
+    iApply (wpc_mono' with "[Hv1] [] H"); last by auto.
+    iIntros (v2) "H". iDestruct "H" as (vs2) "(Hj&Hv2)".
+    simpl.
+
+    iDestruct "Hspec" as "(#Hsrc&#Hstate)".
+    iApply wp_wpc.
+    subst;
+      iDestruct "Hv1" as (?) "(%&%)"; subst;
+      iDestruct "Hv2" as (?) "(%&%)"; subst;
+    (iDestruct (twophase_started_step_puredet with "Hj") as "Hj";
+        [ intros ?; apply head_prim_step_trans'; repeat econstructor; eauto
+        | wp_pures; eauto; iExists _; iFrame; eauto]).
+  (* data *)
+  - subst. simpl.
+    iPoseProof (IHHtyping1 with "[//] [$] [$]") as "H"; eauto.
+    wpc_bind (subst_map ((subst_ival <$> Γsubst)) e1').
+    spec_bind (subst_map ((subst_sval <$> Γsubst)) e1) as Hctx'.
+    iSpecialize ("H" $! j _ _ Hctx' with "Hj").
+    iApply (wpc_mono' with "[] [] H"); last by auto.
+    iIntros (v1) "H". iDestruct "H" as (vs1) "(Hj&Hv1)".
+    clear Hctx'.
+    simpl.
+
+    wpc_bind (subst_map _ e2').
+    spec_bind (subst_map ((subst_sval <$> Γsubst)) e2) as Hctx'.
+    iPoseProof (IHHtyping2 with "[//] [$] [$]") as "H"; eauto.
+    iSpecialize ("H" $! j _ _ Hctx'  with "Hj").
+    iApply (wpc_mono' with "[Hv1] [] H"); last by auto.
+    iIntros (v2) "H". iDestruct "H" as (vs2) "(Hj&Hv2)".
+    simpl.
+    clear Hctx'.
+
+    spec_bind (_ ,_)%E as Hctx'.
+    iApply wp_wpc.
+    iDestruct (twophase_started_step_puredet with "Hj") as "Hj".
+    { intros ?.
+      apply head_prim_step_trans'. repeat econstructor; eauto.
+    }
+    wp_pures; auto.
+    iExists _. iFrame. iExists _, _, _, _. iFrame. eauto.
+  - subst. simpl.
+    iPoseProof (IHHtyping with "[//] [$] [$]") as "H"; eauto.
+    wpc_bind (subst_map ((subst_ival <$> Γsubst)) e').
+    spec_bind (subst_map ((subst_sval <$> Γsubst)) e) as Hctx'.
+    iSpecialize ("H" $! j _ _ Hctx' with "Hj").
+    iApply (wpc_mono' with "[] [] H"); last by auto.
+    iIntros (v) "H". iDestruct "H" as (vs) "(Hj&Hv)".
+    clear Hctx'.
+    simpl.
+    iDestruct "Hv" as (???? (->&->)) "(?&?)".
+
+    iApply wp_wpc.
+    iDestruct (twophase_started_step_puredet with "Hj") as "Hj".
+    { intros ?.
+      apply head_prim_step_trans'. repeat econstructor; eauto.
+    }
+    wp_pures; eauto.
+  - subst. simpl.
+    iPoseProof (IHHtyping with "[//] [$] [$]") as "H"; eauto.
+    wpc_bind (subst_map ((subst_ival <$> Γsubst)) e').
+    spec_bind (subst_map ((subst_sval <$> Γsubst)) e) as Hctx'.
+    iSpecialize ("H" $! j _ _ Hctx' with "Hj").
+    iApply (wpc_mono' with "[] [] H"); last by auto.
+    iIntros (v) "H". iDestruct "H" as (vs) "(Hj&Hv)".
+    clear Hctx'.
+    simpl.
+    iDestruct "Hv" as (???? (->&->)) "(?&?)".
+
+    iApply wp_wpc.
+    iDestruct (twophase_started_step_puredet with "Hj") as "Hj".
+    { intros ?.
+      apply head_prim_step_trans'. repeat econstructor; eauto.
+    }
+    wp_pures; eauto.
+  - subst. simpl.
+    iPoseProof (IHHtyping1 with "[//] [$] [$]") as "H1"; eauto.
+    iPoseProof (IHHtyping2 with "[//] [$] [$]") as "H2"; eauto.
+    wpc_bind (subst_map ((subst_ival <$> Γsubst)) ehd').
+    spec_bind (subst_map ((subst_sval <$> Γsubst)) ehd) as Hctx'.
+    iSpecialize ("H1" $! j _ _ Hctx' with "Hj").
+    iApply (wpc_mono' with "[H2] [] H1"); last by auto.
+    iIntros (v1) "H". iDestruct "H" as (vs1) "(Hj&Hv1)".
+    clear Hctx'.
+    simpl.
+
+    wpc_bind (subst_map ((subst_ival <$> Γsubst)) etl').
+    spec_bind (subst_map ((subst_sval <$> Γsubst)) etl) as Hctx'.
+    iSpecialize ("H2" $! j _ _ Hctx' with "Hj").
+    iApply (wpc_mono' with "[Hv1] [] H2"); last by auto.
+    iIntros (v2) "H". iDestruct "H" as (vs2) "(Hj&Hv2)".
+    clear Hctx'.
+    simpl.
+
+    spec_bind (vs1, vs2)%E as Hctx'.
+    iDestruct (twophase_started_step_puredet _ _ _ _ _ _ _ (λ x : sexpr, K (ectx_language.fill [InjRCtx] x))
+                 with "Hj") as "Hj".
+    { intros ?.
+      apply head_prim_step_trans'. repeat econstructor; eauto.
+    }
+    clear Hctx'.
+    simpl.
+
+    iDestruct (twophase_started_step_puredet with "Hj") as "Hj".
+    { intros ?.
+      apply head_prim_step_trans'. repeat econstructor; eauto.
+    }
+    iApply wp_wpc.
+    wp_pures; auto.
+    iExists _. iFrame.
+    rewrite /atomically_listT_interp.
+    iDestruct "Hv2" as (lvs lv (->&->)) "H".
+    iExists (vs1 :: lvs), (v1 :: lv). iSplit; first by eauto.
+    simpl. iFrame.
+  - subst. simpl.
+    iPoseProof (IHHtyping1 with "[//] [$] [$]") as "H1"; eauto.
+    iPoseProof (IHHtyping2 with "[//] [$] [$]") as "H2"; eauto.
+    iPoseProof (IHHtyping3 with "[//] [$] [$]") as "H3"; eauto.
+    rewrite /impl.ListMatch.
+    wpc_bind (subst_map ((subst_ival <$> Γsubst)) consfun').
+    spec_bind (subst_map ((subst_sval <$> Γsubst)) consfun) as Hctx'.
+    iSpecialize ("H3" $! j _ _ Hctx' with "Hj").
+    iApply (wpc_mono' with "[H1 H2] [] H3"); last by auto.
+    iIntros (vconsfun) "H". iDestruct "H" as (vsconsfun) "(Hj&Hvconsfun)".
+    clear Hctx'.
+    simpl.
+
+    wpc_bind (subst_map ((subst_ival <$> Γsubst)) nilfun').
+    spec_bind (subst_map ((subst_sval <$> Γsubst)) nilfun) as Hctx'.
+    iSpecialize ("H2" $! j _ _ Hctx' with "Hj").
+    iApply (wpc_mono' with "[H1 Hvconsfun] [] H2"); last by auto.
+    iIntros (vnilfun) "H". iDestruct "H" as (vsnilfun) "(Hj&Hvnilfun)".
+    clear Hctx'.
+    simpl.
+
+    wpc_bind (subst_map ((subst_ival <$> Γsubst)) el').
+    spec_bind (subst_map ((subst_sval <$> Γsubst)) el) as Hctx'.
+    iSpecialize ("H1" $! j _ _ Hctx' with "Hj").
+    iApply (wpc_mono' with "[Hvnilfun Hvconsfun] [] H1"); last by auto.
+    iIntros (vl) "H". iDestruct "H" as (vsl) "(Hj&Hvsl)".
+    clear Hctx'.
+    simpl.
+    iApply wp_wpc.
+
+    spec_bind (App _ vsl)%E as Hctx'.
+    iDestruct (twophase_started_step_puredet _ _ _ _ _ _ _
+                 (λ x, K (ectx_language.fill [AppLCtx vsnilfun; AppLCtx vsconsfun] x))  with "Hj") as "Hj".
+    { intros ?.
+      apply head_prim_step_trans'. repeat econstructor; eauto.
+    }
+    wp_pures; eauto.
+    clear Hctx'.
+    simpl.
+
+    spec_bind (λ: _, _)%E as Hctx'.
+    iDestruct (twophase_started_step_puredet _ _ _ _ _ _ _
+                 (λ x, K (ectx_language.fill [AppLCtx vsnilfun; AppLCtx vsconsfun] x))  with "Hj") as "Hj".
+    { intros ?.
+      apply head_prim_step_trans'. repeat econstructor; eauto.
+    }
+    simpl.
+    clear Hctx'.
+
+    spec_bind (App _ vsnilfun)%E as Hctx'.
+    iDestruct (twophase_started_step_puredet _ _ _ _ _ _ _
+                 (λ x, K (ectx_language.fill [AppLCtx vsconsfun] x))  with "Hj") as "Hj".
+    { intros ?.
+      apply head_prim_step_trans'. repeat econstructor; eauto.
+    }
+    clear Hctx'.
+    simpl.
+
+    spec_bind (λ: _, _)%E as Hctx'.
+    iDestruct (twophase_started_step_puredet _ _ _ _ _ _ _
+                 (λ x, K (ectx_language.fill [AppLCtx vsconsfun] x))  with "Hj") as "Hj".
+    { intros ?.
+      apply head_prim_step_trans'. repeat econstructor; eauto.
+    }
+    clear Hctx'.
+    simpl.
+
+    spec_bind (App _ vsconsfun)%E as Hctx'.
+    iDestruct (twophase_started_step_puredet  with "Hj") as "Hj".
+    { intros ?.
+      apply head_prim_step_trans'. repeat econstructor; eauto.
+    }
+    clear Hctx'.
+    simpl.
+
+    iDestruct "Hvsl" as (lvs lv (->&->)) "H".
+    destruct lvs as [|vs lvs];
+    destruct lv as [|v lv]; try (iDestruct "H" as %[]; done).
+
+    * simpl.
+      iDestruct (twophase_started_step_puredet  with "Hj") as "Hj".
+      { intros ?.
+        apply head_prim_step_trans'. repeat econstructor; eauto.
+      }
+
+      spec_bind (Rec BAnon _ (vsnilfun (LitV LitUnit)))%E as Hctx'.
+      iDestruct (twophase_started_step_puredet _ _ _ _ _ _ _
+                   (λ x, K (ectx_language.fill [AppLCtx #()] x)) with "Hj") as "Hj".
+      { intros ?.
+        apply head_prim_step_trans'. repeat econstructor; eauto.
+      }
+      simpl.
+      clear Hctx'.
+
+      iDestruct (twophase_started_step_puredet _ _ _ _ _ _ _
+                   _ with "Hj") as "Hj".
+      { intros ?.
+        apply head_prim_step_trans'. repeat econstructor; eauto.
+      }
+
+      simpl.
+
+      wp_pures.
+      rewrite /atomically_arrowT_interp.
+      iDestruct "Hvnilfun" as (f x e fs xs es (->&->)) "#Hwand".
+      iSpecialize ("Hwand" $! #() #() with "[] Hj").
+      { eauto. }
+      iApply (wpc_wp _ _ _ _ _ True%I).
+      iApply (wpc_mono' with "[] [] Hwand"); last by auto.
+      iIntros (v1) "H". iDestruct "H" as (vs1) "(Hj&Hv1)".
+      iExists _. iFrame.
+    * simpl.
+      iDestruct (twophase_started_step_puredet _ _ _ _ _ _ _
+                   _ with "Hj") as "Hj".
+      { intros ?.
+        apply head_prim_step_trans'. repeat econstructor; eauto.
+      }
+
+      spec_bind (Rec _ _ ((vsconsfun
+                      (Var "p"))))%E as Hctx'.
+      iDestruct (twophase_started_step_puredet _ _ _ _ _ _ _
+                   (λ x : sexpr, K (ectx_language.fill [AppLCtx (vs, val_of_list lvs)] x)) with "Hj") as "Hj".
+      { intros ?.
+        apply head_prim_step_trans'. repeat econstructor; eauto.
+      }
+      simpl.
+      clear Hctx'.
+
+      iDestruct (twophase_started_step_puredet _ _ _ _ _ _ _
+                   _ with "Hj") as "Hj".
+      { intros ?.
+        apply head_prim_step_trans'. repeat econstructor; eauto.
+      }
+      simpl.
+
+      wp_pures.
+      rewrite /atomically_arrowT_interp.
+      iDestruct "Hvconsfun" as (f x e fs xs es (->&->)) "#Hwand".
+      iSpecialize ("Hwand" $! (v, list.val_of_list lv)%V (vs, list.val_of_list lvs)%V with "[H] Hj").
+      { iExists _, _, _, _. iSplit; first by eauto.
+        iDestruct "H" as "($&H)".
+        iExists _, _. iSplit; first eauto. iFrame.
+      }
+      iApply (wpc_wp _ _ _ _ _ True%I).
+      iApply (wpc_mono' with "[] [] Hwand"); last by auto.
+      iIntros (v1) "H". iDestruct "H" as (vs1) "(Hj&Hv1)".
+      iExists _. iFrame.
+  - subst. simpl.
+    iPoseProof (IHHtyping with "[//] [$] [$]") as "H"; eauto.
+    wpc_bind (subst_map ((subst_ival <$> Γsubst)) e').
+    spec_bind (subst_map ((subst_sval <$> Γsubst)) e) as Hctx'.
+    iSpecialize ("H" $! j _ _ Hctx' with "Hj").
+    iApply (wpc_mono' with "[] [] H"); last by auto.
+    iIntros (v1) "H". iDestruct "H" as (vs1) "(Hj&Hv1)".
+    clear Hctx'.
+    simpl.
+
+    simpl.
+    iApply wp_wpc.
+    iDestruct (twophase_started_step_puredet _ _ _ _ _ _ _
+                 _ with "Hj") as "Hj".
+    { intros ?.
+      apply head_prim_step_trans'. repeat econstructor; eauto.
+    }
+    simpl.
+    wp_pures; auto.
+    iExists _. iFrame. iLeft. iExists _, _; iFrame; eauto.
+  - subst. simpl.
+    iPoseProof (IHHtyping with "[//] [$] [$]") as "H"; eauto.
+    wpc_bind (subst_map ((subst_ival <$> Γsubst)) e').
+    spec_bind (subst_map ((subst_sval <$> Γsubst)) e) as Hctx'.
+    iSpecialize ("H" $! j _ _ Hctx' with "Hj").
+    iApply (wpc_mono' with "[] [] H"); last by auto.
+    iIntros (v1) "H". iDestruct "H" as (vs1) "(Hj&Hv1)".
+    clear Hctx'.
+    simpl.
+
+    simpl.
+    iApply wp_wpc.
+    iDestruct (twophase_started_step_puredet _ _ _ _ _ _ _
+                 _ with "Hj") as "Hj".
+    { intros ?.
+      apply head_prim_step_trans'. repeat econstructor; eauto.
+    }
+    wp_pures; auto.
+    iExists _. iFrame. iRight. iExists _, _; iFrame; eauto.
+  - subst. simpl.
+    iPoseProof (IHHtyping1 with "[//] [$] [$]") as "H"; eauto.
+    wpc_bind (subst_map ((subst_ival <$> Γsubst)) cond').
+    spec_bind (subst_map ((subst_sval <$> Γsubst)) cond) as Hctx'.
+    iSpecialize ("H" $! j _ _ Hctx' with "Hj").
+    iApply (wpc_mono' with "[] [] H"); last by auto.
+    iIntros (v1) "H". iDestruct "H" as (vs1) "(Hj&Hv1)".
+    clear Hctx'.
+    simpl.
+
+    iDestruct "Hv1" as "[Hleft|Hright]".
+    {
+      iDestruct "Hleft" as (?? (->&->)) "Hv".
+      wpc_pures; first (iClear "# ∗"; auto).
+      iApply wp_wpc.
+      iDestruct (twophase_started_step_puredet _ _ _ _ _ _ _
+                                               _ with "Hj") as "Hj".
+      { intros ?.
+        apply head_prim_step_trans'. repeat econstructor; eauto.
+      }
+      iApply wpc_wp.
+      wpc_bind (subst_map _ e1').
+      iPoseProof (IHHtyping2 with "[//] [$] [$]") as "H"; eauto.
+      spec_bind (subst_map _ e1) as Hctx'.
+      iSpecialize ("H" $! j _ _ Hctx' with "Hj").
+      iApply (wpc_mono' with "[Hv] [] H"); last first.
+      { iModIntro. iIntros "H". iExact "H". }
+      iIntros (v1) "H". iDestruct "H" as (vs1) "(Hj&Hv1)".
+      simpl. iDestruct "Hv1" as (?????? (Heq1&Heq2)) "#Hinterp".
+      iSpecialize ("Hinterp" with "[$]").
+      iSpecialize ("Hinterp" $! j _ _ Hctx with "Hj").
+      iApply (wpc_mono' with "[] [] Hinterp"); last first.
+      { iModIntro. iIntros "H". iExact "H". }
+      { iIntros (v'') "H". iDestruct "H" as (vs'') "(Hj&Hv')".
+        iExists _. iFrame. }
+    }
+    {
+      iDestruct "Hright" as (?? (->&->)) "Hv".
+      wpc_pures; first (iClear "# ∗"; auto).
+      iApply wp_wpc.
+      iDestruct (twophase_started_step_puredet _ _ _ _ _ _ _
+                                               _ with "Hj") as "Hj".
+      { intros ?.
+        apply head_prim_step_trans'. repeat econstructor; eauto.
+      }
+      iApply (wpc_wp _ _).
+      wpc_bind (subst_map _ e2').
+      iPoseProof (IHHtyping3 with "[//] [$] [$]") as "H"; eauto.
+      spec_bind (subst_map _ e2) as Hctx'.
+      iSpecialize ("H" $! j _ _ Hctx' with "Hj").
+      iApply (wpc_mono' with "[Hv] [] H"); last first.
+      { iModIntro. iIntros "H". iExact "H". }
+      iIntros (v1) "H". iDestruct "H" as (vs1) "(Hj&Hv1)".
+      simpl. iDestruct "Hv1" as (?????? (Heq1&Heq2)) "#Hinterp".
+      iSpecialize ("Hinterp" with "[$]").
+      iSpecialize ("Hinterp" $! j _ _ Hctx with "Hj").
+      iApply (wpc_mono' with "[] [] Hinterp"); last by auto.
+      iIntros (v'') "H". iDestruct "H" as (vs'') "(Hj&Hv')".
+      iExists _. iFrame.
+    }
+  (* Journal operations *)
+  - admit.
+  - admit.
+  (* Value typing *)
+  - admit.
+  - admit.
+  - admit.
+  - admit.
+  - admit.
+  - admit.
+  - admit.
+Admitted.
+
+End reln_defs.
 End reln.
